src/HOL/Word/Word_Examples.thy
@@ -103,8 +103,7 @@ lemma "1 OR 1 = (1 :: byte)" by simp
 lemma "1 XOR 7 = (6 :: byte)" by simp
 lemma "1 XOR 1 = (0 :: byte)" by simp
 lemma "NOT 1 = (254 :: byte)" by simp
-lemma "NOT 0 = (255 :: byte)" apply simp oops
-(* FIXME: "NOT 0" rewrites to "max_word" instead of "-1" *)
+lemma "NOT 0 = (255 :: byte)" by simp
 
 lemma "(-1 :: 32 word) = 0xFFFFFFFF" by simp
 
